update

Loda/Typing.lean
@@ -44,44 +44,72 @@ inductive SubtypeJudgment : Ast.Env -> TyEnv → Option Ast.Ty → Option Ast.Ty
       (∀ i, i < Ts₁.length → SubtypeJudgment σ Γ Ts₁[i]? Ts₂[i]?) →
       SubtypeJudgment σ Γ (pure (Ast.Ty.prod Ts₁)) (pure (Ast.Ty.prod Ts₂))
 
-inductive TypeJudgment: Ast.Env -> Ast.CircuitEnv -> TyEnv -> Ast.Expr -> (Ast.Ty × Ast.Env) -> Prop where
+inductive TypeJudgment: Ast.Env -> Ast.CircuitEnv -> TyEnv -> ℕ -> Ast.Expr -> (Ast.Ty × Ast.Env) -> Prop where
   -- TE-VAR
-  | TE_Var {σ: Ast.Env} {δ: Ast.CircuitEnv} {Γ: TyEnv} {x : String} {v: Ast.Value} {T: Ast.Ty} {φ: Prop}:
+  | TE_Var {σ: Ast.Env} {δ: Ast.CircuitEnv} {Γ: TyEnv} {ctr: ℕ} {x : String} {v: Ast.Value} {T: Ast.Ty} {φ: Prop}:
       Γ x = (Ast.Ty.refin v T φ) →
-    TypeJudgment σ δ Γ (Ast.Expr.var x) ((Ast.Ty.refin v T (v = Ast.eval σ δ (Ast.Expr.var x))), σ)
+    TypeJudgment σ δ Γ ctr (Ast.Expr.var x) ((Ast.Ty.refin v T (v = Ast.eval σ δ ctr (Ast.Expr.var x))), σ)
 
   -- TE-VAR-FUNC
-  | T_VarFunc {σ: Ast.Env} {δ: Ast.CircuitEnv} {Γ: TyEnv} {f x : String} {τ₁ τ₂: Ast.Ty}:
+  | T_VarFunc {σ: Ast.Env} {δ: Ast.CircuitEnv} {Γ: TyEnv} {ctr: ℕ} {f x : String} {τ₁ τ₂: Ast.Ty}:
       Γ f = (Ast.Ty.func x τ₁ τ₂) →
-      TypeJudgment σ δ Γ (Ast.Expr.var f) ((Ast.Ty.func x τ₁ τ₂), σ)
+      TypeJudgment σ δ Γ ctr (Ast.Expr.var f) ((Ast.Ty.func x τ₁ τ₂), σ)
 
   -- TE-NONDET
-  | T_Nondet {σ: Ast.Env} {δ: Ast.CircuitEnv} {Γ: TyEnv} {p: ℕ} {v: Ast.Value}:
-    TypeJudgment σ δ Γ Ast.Expr.wildcard ((Ast.Ty.refin v (Ast.Ty.field p) True), σ)
+  | T_Nondet {σ: Ast.Env} {δ: Ast.CircuitEnv} {Γ: TyEnv} {ctr: ℕ} {p: ℕ} {v: Ast.Value}:
+    TypeJudgment σ δ Γ ctr Ast.Expr.wildcard ((Ast.Ty.refin v (Ast.Ty.field p) True), σ)
 
   -- TE-CONSTF
-  | T_ConstF {σ: Ast.Env} {δ: Ast.CircuitEnv} {Γ: TyEnv} {p: ℕ} {v: Ast.Value} {f: F p} :
-    TypeJudgment σ δ Γ (Ast.Expr.constF p f) ((Ast.Ty.refin v (Ast.Ty.field p) (v = Ast.Value.vF p f)), σ)
+  | T_ConstF {σ: Ast.Env} {δ: Ast.CircuitEnv} {Γ: TyEnv} {ctr: ℕ} {p: ℕ} {v: Ast.Value} {f: F p} :
+    TypeJudgment σ δ Γ ctr (Ast.Expr.constF p f) ((Ast.Ty.refin v (Ast.Ty.field p) (v = Ast.Value.vF p f)), σ)
 
   -- TE-ASSERT
-  | T_Assert {σ: Ast.Env} {δ: Ast.CircuitEnv} {Γ: TyEnv} {e₁ e₂: Ast.Expr} {p: ℕ} {v: Ast.Value} :
-    TypeJudgment σ δ Γ e₁ ((Ast.Ty.field p), σ) →
-    TypeJudgment σ δ Γ e₂ ((Ast.Ty.field p), σ) →
-    TypeJudgment σ δ Γ (Ast.Expr.assertE e₁ e₂) ((Ast.Ty.refin v Ast.Ty.unit (Ast.eval σ δ e₁ = Ast.eval σ δ e₂)), σ)
+  | T_Assert {σ: Ast.Env} {δ: Ast.CircuitEnv} {Γ: TyEnv} {ctr: ℕ} {e₁ e₂: Ast.Expr} {p: ℕ} {v: Ast.Value} :
+    TypeJudgment σ δ Γ ctr e₁ ((Ast.Ty.field p), σ) →
+    TypeJudgment σ δ Γ ctr e₂ ((Ast.Ty.field p), σ) →
+    TypeJudgment σ δ Γ ctr (Ast.Expr.assertE e₁ e₂) ((Ast.Ty.refin v Ast.Ty.unit (Ast.eval σ δ ctr e₁ = Ast.eval σ δ ctr e₂)), σ)
 
   -- TE-BINOPFIELD
-  | T_BinOpField {σ: Ast.Env} {δ: Ast.CircuitEnv} {Γ: TyEnv} {e₁ e₂: Ast.Expr} {op: Ast.FieldOp} {p: ℕ} {v: Ast.Value}:
-    TypeJudgment σ δ Γ e₁ ((Ast.Ty.field p), σ) →
-    TypeJudgment σ δ Γ e₂ ((Ast.Ty.field p), σ) →
-    TypeJudgment σ δ Γ (Ast.Expr.fieldExpr e₁ op e₂) ((Ast.Ty.refin v (Ast.Ty.field p) (v = Ast.eval σ δ (Ast.Expr.fieldExpr e₁ op e₂))), σ)
+  | T_BinOpField {σ: Ast.Env} {δ: Ast.CircuitEnv} {Γ: TyEnv} {ctr: ℕ} {e₁ e₂: Ast.Expr} {op: Ast.FieldOp} {p: ℕ} {v: Ast.Value}:
+    TypeJudgment σ δ Γ ctr e₁ ((Ast.Ty.field p), σ) →
+    TypeJudgment σ δ Γ ctr e₂ ((Ast.Ty.field p), σ) →
+    TypeJudgment σ δ Γ ctr (Ast.Expr.fieldExpr e₁ op e₂) ((Ast.Ty.refin v (Ast.Ty.field p) (v = Ast.eval σ δ ctr (Ast.Expr.fieldExpr e₁ op e₂))), σ)
 
   -- TE-ABS (function abstraction)
-  | T_Abs {σ: Ast.Env} {δ: Ast.CircuitEnv} {Γ: TyEnv} {x: String} {τ₁ τ₂: Ast.Ty} {e: Ast.Expr}:
-    TypeJudgment σ δ (setTy Γ x τ₁) e (τ₂, σ) →
-    TypeJudgment σ δ Γ (Ast.Expr.lam x τ₁ e) ((Ast.Ty.func x τ₁ τ₂), σ)
+  | T_Abs {σ: Ast.Env} {δ: Ast.CircuitEnv} {Γ: TyEnv} {ctr: ℕ} {x: String} {τ₁ τ₂: Ast.Ty} {e: Ast.Expr}:
+    TypeJudgment σ δ (setTy Γ x τ₁) ctr e (τ₂, σ) →
+    TypeJudgment σ δ Γ ctr (Ast.Expr.lam x τ₁ e) ((Ast.Ty.func x τ₁ τ₂), σ)
 
   -- TE-APP
-  | T_App {σ: Ast.Env} {δ: Ast.CircuitEnv} {Γ: TyEnv} {x₁ x₂: Ast.Expr} {s: String} {τ₁ τ₂: Ast.Ty} {v: Ast.Value}:
-    TypeJudgment σ δ Γ x₁ ((Ast.Ty.func s τ₁ τ₂), σ) →
-    Ast.eval σ δ x₂ = some v →
-    TypeJudgment σ δ Γ x₂ (τ₁, σ) → TypeJudgment σ δ Γ (Ast.Expr.app x₁ x₂) (τ₂, (Ast.set σ s v))
+  | T_App {σ: Ast.Env} {δ: Ast.CircuitEnv} {Γ: TyEnv} {ctr: ℕ} {x₁ x₂: Ast.Expr} {s: String} {τ₁ τ₂: Ast.Ty} {v: Ast.Value}:
+    TypeJudgment σ δ Γ ctr x₁ ((Ast.Ty.func s τ₁ τ₂), σ) →
+    Ast.eval σ δ ctr x₂ = some v →
+    TypeJudgment σ δ Γ ctr x₂ (τ₁, σ) → TypeJudgment σ δ Γ ctr (Ast.Expr.app x₁ x₂) (τ₂, (Ast.set σ s v))
+
+open Ast
+-- dummy environments
+def σ0 : Env := fun _ => Value.vBool true
+def Γ0 : TyEnv := fun _ => Ty.int
+def Γ1 := setTy Γ0 "x" Ty.bool
+def δ0 : Ast.CircuitEnv :=
+  fun _ => { name := "idInt", inputs := [("x", Ast.Ty.int)], output := Ast.Ty.int,
+                 body := Ast.Expr.var "x" }
+
+example : SubtypeJudgment σ0 Γ0 (pure Ty.int) (pure Ty.int) :=
+  SubtypeJudgment.TSub_Refl
+
+-- refinement subtyping: {v:int | True} <: {v:int | True}
+example : SubtypeJudgment σ0 Γ0 (pure (Ty.refin (Value.vInt 1) Ty.int (True))) (pure (Ty.refin (Value.vInt 1) Ty.int (True))) := by
+  apply SubtypeJudgment.TSub_Refine
+  · apply SubtypeJudgment.TSub_Refl
+  · intros _; trivial
+
+-- TypeJudgment tests
+
+def tyEnv : TyEnv := fun
+  | "b" => Ty.bool
+  | "f" => Ty.func "x" Ty.int Ty.bool
+  | _   => Ty.int
+
+-- TE_VAR: assume env maps "b" to {v | v = eval ...}
+example : TypeJudgment σ0 δ0 Γ0 (Expr.var "b") ((Ty.refin (Value.vBool true) Ty.bool (Value.vBool true = eval σ0 δ0 123 (Expr.var "b"))), σ0) := by
